Test/civl/async/inc-dec.bpl
@@ -12,13 +12,13 @@ var {:layer 0,1} x : int;
 // ###########################################################################
 // Main
 
-procedure {:yields} {:layer 1} main ()
+yield procedure {:layer 1} main ()
 {
   async call {:sync} inc_by_N();
   async call {:sync} dec_by_N();
 }
 
-procedure {:yields} {:layer 1} {:left} inc_by_N ()
+yield <- procedure {:layer 1} inc_by_N ()
 modifies x;
 ensures {:layer 1} x == old(x) + N;
 {
@@ -33,7 +33,7 @@ ensures {:layer 1} x == old(x) + N;
   }
 }
 
-procedure {:yields} {:layer 1} {:left} dec_by_N ()
+yield <- procedure {:layer 1} dec_by_N ()
 modifies x;
 ensures {:layer 1} x == old(x) - N;
 {
@@ -51,13 +51,13 @@ ensures {:layer 1} x == old(x) - N;
 // ###########################################################################
 // Low level atomic actions
 
-procedure {:left} {:layer 1} inc_atomic ()
+<- action {:layer 1} inc_atomic ()
 modifies x;
 { x := x + 1; }
 
-procedure {:left} {:layer 1} dec_atomic ()
+<- action {:layer 1} dec_atomic ()
 modifies x;
 { x := x - 1; }
 
-procedure {:yields} {:layer 0} {:refines "inc_atomic"} inc ();
-procedure {:yields} {:layer 0} {:refines "dec_atomic"} dec ();
+yield procedure {:layer 0} inc () refines inc_atomic;
+yield procedure {:layer 0} dec () refines dec_atomic;
